lots of polishing

Semantics/Dynamic/Bool.v
@@ -11,212 +11,37 @@ From ExtensibleCompiler.Theory Require Import ProofAlgebra.
 From ExtensibleCompiler.Theory Require Import ProgramAlgebra.
 From ExtensibleCompiler.Theory Require Import SubFunctor.
 From ExtensibleCompiler.Theory Require Import Types.
+From ExtensibleCompiler.Theory Require Import TypeSoundness.
 From ExtensibleCompiler.Theory Require Import UniversalProperty.
 
 Local Open Scope SubFunctor_scope.
 
-Definition eval_Bool
-           {O} `{FunctorLaws O} `{! SubFunctor Bool O}
-           (R : Set) (rec : R -> Fix O)
-           (e : Bool R)
-  : Fix O
-  := match e with MkBool b => boolean b end.
+Definition eval__Bool
+           {V} `{FunctorLaws V}
+           `{! V supports Bool}
+  : forall {T}, MixinAlgebra Bool T (WellFormedValue V)
+  := fun _ rec '(MkBool b) => boolean b.
 
-Global Instance Eval_Bool__WF
-       {O} `{FunctorLaws O}
-       `{! SubFunctor Bool O}
-       T
-  : ProgramAlgebra Bool T (WellFormedValue O)
-  | 0 :=
-  {| programAlgebra := fun rec '(MkBool b) => boolean' b; |}.
+Global Instance EvalAlgebra__Bool
+       {V} `{FunctorLaws V}
+       `{! SubFunctor Bool V}
+  : forall {T}, ProgramAlgebra Bool T (WellFormedValue V)
+  := fun _ => {| programAlgebra := eval__Bool; |}.
 
-Definition eval_Bool_1 (e : Fix Bool) : WellFormedValue Bool
-  := mendlerFold (fun _ => programAlgebra) e.
-
-Global Instance Eval_Bool__Fix
-       {O} `{FunctorLaws O}
-       `{! SubFunctor Bool O}
-       T
-  : ProgramAlgebra Bool T (Fix O)
-  | 0 :=
-  {| programAlgebra := eval_Bool T; |}.
-
-Inductive Eval_Bool {E V}
+Inductive Eval__Bool {E V}
           `{FunctorLaws E} `{FunctorLaws V}
           `{! SubFunctor Bool E} `{! SubFunctor Bool V}
           (Eval_E : (WellFormedValue E * WellFormedValue V) -> Prop)
   : (WellFormedValue E * WellFormedValue V) -> Prop
   :=
-  | BoolValue : forall b, Eval_Bool Eval_E (boolean' b, boolean' b)
+  | BoolValue : forall b, Eval__Bool Eval_E (boolean b, boolean b)
 .
 
-Record WFValue_i
-       V LT
-       `{FunctorLaws V}
-       `{FunctorLaws LT}
-  : Set :=
-    mk_WFValue_i { wfv_a : UniversalPropertyF V; wfv_b : UniversalPropertyF LT; }.
-
-(**
-In MTC, this is parameterized by some indexed relation.  In practice I don't
-think I am using it yet, so leaving it hardcoded until it becomes necessary.
-*)
-
-Definition WFValue
-           V LT
-           `{FunctorLaws V} `{FunctorLaws LT}
-           (* WFV : (WFValue_i V LT -> Prop) -> WFValue_i V LT -> Prop *)
-  : WFValue_i V LT -> Prop
-  := IndexedFix (fun _ _ => True) (* should be WFV *).
-
-Definition WFValueC
-           {V LT}
-           `{FunctorLaws V} `{FunctorLaws LT}
-           (*WFV : (WFValue_i V LT)-relation*)
-           v lt
-  := WFValue V LT (*WFV*) (mk_WFValue_i V LT _ _ _ _ v lt).
-
-(**
-This is the most abstract statement of the type soundness of evaluation.
-
-Instead of explicitly calling recursively [evalL] and [typeOfL], this is
-abstracted over the operation to run recursively, namely [recEval] and
-[recTypeOf].
-
- *)
-
-Definition eval_alg_Soundness_P
-           {L L' LT V}
-           `{FunctorLaws L} `{FunctorLaws L'} `{FunctorLaws LT} `{FunctorLaws V}
-           (*WFV : (WFValue_i V LT -> Prop) -> WFValue_i V LT -> Prop*)
-           `{evalL   : forall {T}, MixinAlgebra T L (EvalResult V)}
-           `{typeOfL : forall {T}, MixinAlgebra T L' (TypeOfResult LT)}
-           (recEval : UniversalPropertyF L -> EvalResult V)
-           (recTypeOf : UniversalPropertyF L' -> TypeOfResult LT)
-           (e : Fix L' * Fix L)
-           (RFUP_e : ReverseFoldUniversalProperty (fst e) /\ ReverseFoldUniversalProperty (snd e))
-  : Prop
-  :=
-    forall
-
-      (* Commenting those out temporarily to see where they are needed! *)
-
-      (* recEvalProj : forall (e : UniversalPropertyF L),
-          recEval e
-          =
-          recEval (reverseFoldWrapFix (reverseFoldUnwrapFix (proj1_sig e)))
-      *)
-
-      (* recTypeOfProj : forall (e : UniversalPropertyF L'),
-          recTypeOf e
-          =
-          recTypeOf (reverseFoldWrapFix (reverseFoldUnwrapFix (proj1_sig e)))
-      *)
-
-      (IH : forall (a : UniversalPropertyF L' * UniversalPropertyF L),
-          (forall T,
-              typeOfL recTypeOf (reverseFoldUnwrapFix (proj1_sig (fst a))) = Some T ->
-              WFValueC (*WFV*) (evalL recEval (reverseFoldUnwrapFix (proj1_sig (snd a)))) T
-          ) ->
-          forall T,
-            recTypeOf (fst a) = Some T ->
-            WFValueC (*WFV*) (recEval (reverseFoldWrapFix (reverseFoldUnwrapFix (proj1_sig (snd a))))) T
-      )
-    ,
-    forall (T : TypeFix LT),
-      typeOfL recTypeOf (reverseFoldUnwrapFix (fst e)) = Some T ->
-      WFValueC (*WFV*) (evalL recEval (reverseFoldUnwrapFix (snd e))) T.
-
-Definition Eval_Soundness_alg_F
-           {L LT V}
-           `{FunctorLaws L} `{FunctorLaws LT} `{FunctorLaws V}
-           (WFV : (WFValue_i V LT -> Prop) -> WFValue_i V LT -> Prop)
-           `{EvalL   : forall {T}, ProgramAlgebra L T (EvalResult V)}
-           `{TypeOfL : forall {T}, ProgramAlgebra L T (TypeOfResult LT)}
-  := forall recTypeOf recEval,
-    ProofAlgebra
-      L
-      (sig
-         (UniversalPropertyP2
-            (eval_alg_Soundness_P
-               (evalL   := fun _ => programAlgebra' EvalL)
-               (typeOfL := fun _ => programAlgebra' TypeOfL)
-               (*fun _ _ => True*)
-               recTypeOf recEval
-      ))).
-
-Definition eval_Soundness_P
-           {L LT V}
-           `{FunctorLaws L} `{FunctorLaws LT} `{FunctorLaws V}
-           (*WFV : (WFValue_i V LT -> Prop) -> WFValue_i V LT -> Prop*)
-           `{EvalL   : forall {T}, ProgramAlgebra L T (EvalResult V)}
-           `{TypeOfL : forall {T}, ProgramAlgebra L T (TypeOfResult LT)}
-           (recEval : UniversalPropertyF L -> EvalResult V)
-           (recTypeOf : UniversalPropertyF L -> TypeOfResult LT)
-           (e : Fix L)
-           (RFUP_e : ReverseFoldUniversalProperty e)
-  : Prop
-  :=
-    forall (T : TypeFix LT),
-      typeOf e = Some T ->
-      WFValueC (*WFV*) (eval e) T.
-
-Lemma eval_Soundness
-      {L LT V}
-      `{FunctorLaws L} `{FunctorLaws LT} `{FunctorLaws V}
-      (*WFV : (WFValue_i V LT -> Prop) -> WFValue_i V LT -> Prop*)
-      `{EvalL   : forall {T}, ProgramAlgebra L T (EvalResult V)}
-      `{TypeOfL : forall {T}, ProgramAlgebra L T (TypeOfResult LT)}
-      `{WFEvalL : ! WellFormedMendlerAlgebra (@EvalL)}
-      (eval_Soundness_alg_F
-       : Eval_Soundness_alg_F
-           (fun (_ : WFValue_i V LT -> Prop) (_ : WFValue_i V LT) => True) (* should be WFV*)
-      )
-      (WF_eval_Soundness_alg_F :
-         forall recTypeOf recEval,
-           WellFormedProofAlgebra2 (eval_Soundness_alg_F recTypeOf recEval)
-      )
-  : forall (e : WellFormedValue L) (T : TypeFix LT),
-    typeOf (proj1_sig e) = Some T ->
-    WFValueC (*fun _ _ => True*) (eval (proj1_sig e)) T.
-Proof.
-  move => e T TO.
-  setoid_rewrite <- reverseFoldWrapUnwrapFix_inverse.
-  {
-    rewrite // / eval / mendlerFold / reverseFoldWrapFix / wrapFix /=.
-    setoid_rewrite wellFormedMendlerAlgebra.
-    rewrite / mendlerFold.
-    elim (
-        Induction2
-          (PA :=
-             eval_Soundness_alg_F
-               (fun e => eval (proj1_sig e))
-               (fun e => typeOf (proj1_sig e))
-          )
-          _
-          (proj2_sig e)
-      ).
-    rewrite / eval_alg_Soundness_P.
-    move => e' E'.
-    eapply E'.
-    move => [[f F][g G]].
-    rewrite reverseFoldWrapUnwrapFix_inverse /=.
-    rewrite / eval / mendlerFold / reverseFoldUnwrapFix / programAlgebra'.
-    admit.
-Admitted.
-
-Definition blit'
-           {L}
-           `{FunctorLaws L}
-           `{! SubFunctor Bool L}
-           (b : bool)
-  : UniversalPropertyF L :=
-  injectUniversalProperty (MkBool b).
-
-Global Instance Soundness_Eval_Bool
+Global Instance EvalSoundness__Bool
        {L LT V}
        `{FunctorLaws L} `{FunctorLaws LT} `{FunctorLaws V}
        `{! SubFunctor Bool L}
+       (WT : (WellTypedValue V LT -> Prop) -> WellTypedValue V LT -> Prop)
        `{Eval_L   : forall {T}, ProgramAlgebra L T (EvalResult   V)}
        `{TypeOf_L : forall {T}, ProgramAlgebra L T (TypeOfResult LT)}
        (recEval   : UniversalPropertyF L -> EvalResult   V)
@@ -224,7 +49,7 @@ Global Instance Soundness_Eval_Bool
   : ProofAlgebra Bool
       (sig
          (UniversalPropertyP2
-            (eval_alg_Soundness_P (*fun _ _ => True*)
+            (eval_alg_Soundness_P WT
                (evalL   := fun _ => programAlgebra' Eval_L)
                (typeOfL := fun _ => programAlgebra' TypeOf_L)
                recEval recTypeOf
@@ -234,8 +59,8 @@ Proof.
   pose proof (
          Induction2Algebra_Bool
            (@eval_alg_Soundness_P
-              _ _ _ _ _ _ _ _ _ _ _
-              _
+              _ _ _ _ _ _ _ _ _ _ _ _
+              WT
               (fun _ => programAlgebra' (Eval_L   _))
               (fun _ => programAlgebra' (TypeOf_L _))
               recEval
@@ -247,7 +72,7 @@ Proof.
   rewrite / eval_alg_Soundness_P / UniversalPropertyP2.
   constructor => /=.
   {
-    apply conj; apply : (proj2_sig (boolean' b)).
+    apply conj; apply : (proj2_sig (boolean b)).
   }
   {
     admit.
