Syntax/Terms/If2.v
@@ -16,7 +16,6 @@ From ExtensibleCompiler.Theory Require Import Types.
 From ExtensibleCompiler.Theory Require Import UniversalProperty.
 
 Local Open Scope SubFunctor_scope.
-Local Open Scope Sum1_scope.
 
 Inductive If2 (A : Set) : Set :=
 | MkIf2 (condition : A) (thenBranch : A) (elseBranch : A)
@@ -24,30 +23,56 @@ Inductive If2 (A : Set) : Set :=
 Arguments MkIf2 {A}.
 
 Global Instance Functor_If2 : Functor If2 :=
-  {|
-    fmap := fun A B f '(MkIf2 c t e) => MkIf2 (f c) (f t) (f e);
-  |}.
+  {| fmap := fun A B f '(MkIf2 c t e) => MkIf2 (f c) (f t) (f e); |}.
 
 Global Instance FunctorLaws_If2 : FunctorLaws If2.
 Proof.
   constructor.
-  {
-    intros A [].
-    reflexivity.
-  }
-  {
-    intros A B C f g [].
-    reflexivity.
-  }
+  - move => ? [] //.
+  - move => ????? [] //.
 Qed.
 
-Definition if2'
+Definition if2
            {L} `{FunctorLaws L} `{SubFunctor If2 L}
            (condition thenBranch elseBranch : UniversalPropertyF L)
   : UniversalPropertyF L
   := injectUniversalProperty (MkIf2 condition thenBranch elseBranch).
 
-Definition if2__UPP
+Definition if2_Fix_UPF
+           {L} `{FunctorLaws L} `{SubFunctor If2 L}
+           (condition thenBranch elseBranch : Fix L)
+           {H_condition  : ReverseFoldUniversalProperty condition}
+           {H_thenBranch : ReverseFoldUniversalProperty thenBranch}
+           {H_elseBranch : ReverseFoldUniversalProperty elseBranch}
+  : UniversalPropertyF L
+  := if2
+       (exist _ _ H_condition)
+       (exist _ _ H_thenBranch)
+       (exist _ _ H_elseBranch).
+
+Definition if2_Fix_Fix
+           {L} `{FunctorLaws L} `{SubFunctor If2 L}
+           (condition thenBranch elseBranch : Fix L)
+           {H_condition  : ReverseFoldUniversalProperty condition}
+           {H_thenBranch : ReverseFoldUniversalProperty thenBranch}
+           {H_elseBranch : ReverseFoldUniversalProperty elseBranch}
+  : Fix L
+  := proj1_sig (if2_Fix_UPF condition thenBranch elseBranch).
+
+Definition if2_UPP_UPF
+           {L} `{FunctorLaws L} `{SubFunctor If2 L}
+           {condition thenBranch elseBranch : Fix L}
+           {P}
+           (H_condition  : UniversalPropertyP P condition)
+           (H_thenBranch : UniversalPropertyP P thenBranch)
+           (H_elseBranch : UniversalPropertyP P elseBranch)
+  : UniversalPropertyF L
+  := if2_Fix_UPF condition thenBranch elseBranch
+       (H_condition  := proj1_sig H_condition)
+       (H_thenBranch := proj1_sig H_thenBranch)
+       (H_elseBranch := proj1_sig H_elseBranch).
+
+Definition if2_UPP_Fix
            {L} `{FunctorLaws L} `{SubFunctor If2 L}
            {condition thenBranch elseBranch : Fix L}
            {P}
@@ -55,102 +80,34 @@ Definition if2__UPP
            (H_thenBranch : UniversalPropertyP P thenBranch)
            (H_elseBranch : UniversalPropertyP P elseBranch)
   : Fix L
-  := proj1_sig (if2'
-                  (exist _ _ (proj1_sig H_condition))
-                  (exist _ _ (proj1_sig H_thenBranch))
-                  (exist _ _ (proj1_sig H_elseBranch))
-               ).
+  := proj1_sig (if2_UPP_UPF H_condition H_thenBranch H_elseBranch).
 
-Definition if2
-           {L} `{FunctorLaws L} `{SubFunctor If2 L}
-           (condition thenBranch elseBranch : Fix L)
-           {H_condition  : ReverseFoldUniversalProperty condition}
-           {H_thenBranch : ReverseFoldUniversalProperty thenBranch}
-           {H_elseBranch : ReverseFoldUniversalProperty elseBranch}
-  : Fix L
-  := proj1_sig (if2'
-                  (exist _ _ H_condition)
-                  (exist _ _ H_thenBranch)
-                  (exist _ _ H_elseBranch)
-               ).
-
-Global Instance EvalIf2
-       {O} `{FunctorLaws O}
-       `{! SubFunctor Bool  O}
-       `{! SubFunctor Stuck O}
-       T
-  : ProgramAlgebra If2 T (WellFormedValue O)
-  | 0 :=
-  {|
-    programAlgebra :=
-      fun rec '(MkIf2 condition thenBranch elseBranch) =>
-        match project (proj1_sig (rec condition)) with
-        | Some (MkBool b) =>
-          if b
-          then rec thenBranch
-          else rec elseBranch
-        | None => stuck "The condition of a binary branch was not a boolean"
-        end
-    ;
-  |}.
-
-Global Instance EvalIf2Fix
-       {O} `{Functor O} `{FunctorLaws O}
-       `{! SubFunctor Bool  O}
-       `{! SubFunctor Stuck O}
-       T
-  : ProgramAlgebra If2 T (Fix O)
-  | 0 :=
-  {|
-    programAlgebra :=
-      fun rec '(MkIf2 condition thenBranch elseBranch) =>
-        match project (rec condition) with
-        | Some (MkBool b) =>
-          if b
-          then rec thenBranch
-          else rec elseBranch
-        | None =>
-          proj1_sig
-            (
-              stuck "The condition of a binary branch was not a boolean"
-            )
-        end
-    ;
-  |}.
-
-Inductive EvalIf2__WF {E V}
-          `{FunctorLaws E} `{FunctorLaws V}
-          `{! SubFunctor If2   E}
-          `{! SubFunctor Bool V}
-          `{! SubFunctor Unit V}
-          (Eval : (WellFormedValue E * WellFormedValue V) -> Prop)
-  : (WellFormedValue E * WellFormedValue V) -> Prop
-  :=
-  | If2True : forall c t e t',
-      Eval (c, boolean' true) ->
-      Eval (t, t') ->
-      EvalIf2__WF Eval (if2' c t e, t')
-  | If2alse : forall c t e e',
-      Eval (c, boolean' false) ->
-      Eval (e, e') ->
-      EvalIf2__WF Eval (if2' c t e, e')
-.
+(* Definition if2_UP_Fix *)
+(*            {L} `{FunctorLaws L} `{SubFunctor If2 L} *)
+(*            {condition thenBranch elseBranch : Fix L} *)
+(*            (H_condition  : ReverseFoldUniversalProperty condition) *)
+(*            (H_thenBranch : ReverseFoldUniversalProperty thenBranch) *)
+(*            (H_elseBranch : ReverseFoldUniversalProperty elseBranch) *)
+(*   : Fix L *)
+(*   := proj1_sig (if2 *)
+(*                   (exist _ _ H_condition) *)
+(*                   (exist _ _ H_thenBranch) *)
+(*                   (exist _ _ H_elseBranch) *)
+(*                ). *)
 
 Definition If2Induction
            {F} `{FunctorLaws F} `{S : SubFunctor If2 F}
            (P : forall (e : Fix F), ReverseFoldUniversalProperty e -> Prop)
-           (Hif2 : forall c t e
+           (Hif2 : forall (c t e : Fix F)
                      (H_c : UniversalPropertyP P c)
                      (H_t : UniversalPropertyP P t)
                      (H_e : UniversalPropertyP P e),
-               UniversalPropertyP P (if2__UPP H_c H_t H_e))
+               UniversalPropertyP P (if2_UPP_Fix H_c H_t H_e))
   : Algebra If2 (sig (UniversalPropertyP P))
   := fun e =>
        match e with
        | MkIf2 c t e =>
-         exist _
-               (if2 (proj1_sig c) (proj1_sig t) (proj1_sig e))
-               (Hif2 _ _ _ (proj2_sig c) (proj2_sig t) (proj2_sig e))
+         exist _ _ (Hif2 _ _ _ (proj2_sig c) (proj2_sig t) (proj2_sig e))
        end.
 
 (** NOTE: we don't let [SubFunctor] introduce implicitly because it would
@@ -163,7 +120,7 @@ Global Instance If2ProofAlgebra
                    (H_c : UniversalPropertyP P c)
                    (H_t : UniversalPropertyP P t)
                    (H_e : UniversalPropertyP P e),
-            UniversalPropertyP P (if2__UPP H_c H_t H_e))
+            UniversalPropertyP P (if2_UPP_Fix H_c H_t H_e))
   : ProofAlgebra If2 (sig (UniversalPropertyP P))
   := {| proofAlgebra := If2Induction P H_if2; |}.
 
@@ -174,14 +131,14 @@ Global Instance If2ProofAlgebraWellFormed
                    (IH_c : UniversalPropertyP P c)
                    (IH_t : UniversalPropertyP P t)
                    (IH_e : UniversalPropertyP P e),
-            UniversalPropertyP P (if2 c t e)
+            UniversalPropertyP P (if2_Fix_Fix c t e)
         )
   : WellFormedProofAlgebra (If2ProofAlgebra P H_if2).
 Proof.
   constructor.
   rewrite /= / If2Induction.
   move => [] c t e /=.
-  rewrite / if2 / if2 / injectUniversalProperty /=.
+  rewrite / if2_UPP_Fix / if2 / if2 / injectUniversalProperty /=.
   erewrite wellFormedSubFunctor => /=.
   reflexivity.
 Qed.
