Semantics/Dynamic/Unit.v
@@ -1,0 +1,35 @@
+From Coq Require Import String.
+
+From ExtensibleCompiler.Syntax.Terms Require Import Unit.
+
+From ExtensibleCompiler.Theory Require Import Algebra.
+From ExtensibleCompiler.Theory Require Import Eval.
+From ExtensibleCompiler.Theory Require Import Functor.
+From ExtensibleCompiler.Theory Require Import ProgramAlgebra.
+From ExtensibleCompiler.Theory Require Import SubFunctor.
+From ExtensibleCompiler.Theory Require Import UniversalProperty.
+
+Local Open Scope SubFunctor_scope.
+
+Definition eval__Unit
+           {V} `{FunctorLaws V}
+           `{S : ! SubFunctor Unit V}
+  : forall {T}, MixinAlgebra Unit T (WellFormedValue V)
+  := fun T rec '(MkUnit) => unit.
+
+Global Instance EvalAlgebra__Unit
+       {V} `{FunctorLaws V}
+       `{S : ! V supports Unit}
+  : forall {T}, ProgramAlgebra Unit T (WellFormedValue V)
+  := fun T => {| programAlgebra := eval__Unit; |}.
+
+Inductive Eval__Unit
+          {L V}
+          `{FunctorLaws L} `{FunctorLaws V}
+          `{! L supports Unit}
+          `{! V supports Unit}
+          (Eval : (WellFormedValue L * WellFormedValue V) -> Prop)
+  : (WellFormedValue L * WellFormedValue V) -> Prop
+  :=
+  | UnitValue : Eval__Unit Eval (unit, unit)
+.
