Theory/IndexedSum1.v
@@ -3,7 +3,7 @@ From ExtensibleCompiler.Theory Require Import IndexedFunctor.
 Delimit Scope IndexedSum1_scope with IndexedSum1.
 Open Scope IndexedSum1_scope.
 
-Variant IndexedSum1 I (F G : I-relation) (A : I -> Prop) (i : I) : Prop :=
+Variant IndexedSum1 I (F G : I-indexedProp) (A : I -> Prop) (i : I) : Prop :=
 | iinl1 : F A i -> (F + G)%IndexedSum1 A i
 | iinr1 : G A i -> (F + G)%IndexedSum1 A i
 where "F + G" := (IndexedSum1 _ F G) : IndexedSum1_scope.
@@ -11,7 +11,7 @@ Arguments iinl1 {I F G A i}.
 Arguments iinr1 {I F G A i}.
 
 Global Instance IndexedFunctorSum1
-       {I} {F G : I-relation} `{IndexedFunctor I F} `{IndexedFunctor I G}
+       {I} {F G : I-indexedProp} `{IndexedFunctor I F} `{IndexedFunctor I G}
   : IndexedFunctor I (F + G)
   | 0 :=
   {|
@@ -24,7 +24,7 @@ Global Instance IndexedFunctorSum1
   |}.
 
 Definition indexedSum1Dispatch
-           {I} {A : I -> Prop} {L R : I-relation} {O : I -> Prop} {i}
+           {I} {A : I -> Prop} {L R : I-indexedProp} {O : I -> Prop} {i}
            (fl : L A i -> O i) (fr : R A i -> O i) v :=
   match v with
   | iinl1 l => fl l
