Theory/TypeSoundness.v
@@ -1,0 +1,169 @@
+From Coq Require Import ssreflect.
+
+From ExtensibleCompiler.Theory Require Import Algebra.
+From ExtensibleCompiler.Theory Require Import Eval.
+From ExtensibleCompiler.Theory Require Import Functor.
+From ExtensibleCompiler.Theory Require Import IndexedAlgebra.
+From ExtensibleCompiler.Theory Require Import IndexedFunctor.
+From ExtensibleCompiler.Theory Require Import ProofAlgebra.
+From ExtensibleCompiler.Theory Require Import ProgramAlgebra.
+From ExtensibleCompiler.Theory Require Import SubFunctor.
+From ExtensibleCompiler.Theory Require Import Types.
+From ExtensibleCompiler.Theory Require Import UniversalProperty.
+
+Local Open Scope SubFunctor_scope.
+
+Record WellTypedValue (* cf. WellTypedValue *)
+       V LT `{FunctorLaws V} `{FunctorLaws LT}
+  : Set
+  := MkWellTypedValue (* cf. mk_WellTypedValue *)
+       {
+         wellFormedValue : UniversalPropertyF V;
+         wellFormedType  : UniversalPropertyF LT;
+       }.
+
+(**
+In MTC, this is parameterized by some indexed relation.  In practice I don't
+think I am using it yet, so leaving it hardcoded until it becomes necessary.
+*)
+
+Definition WFValue
+           V LT
+           `{FunctorLaws V} `{FunctorLaws LT}
+           (WT : (WellTypedValue V LT)-indexedProp)
+  : WellTypedValue V LT -> Prop
+  := IndexedFix WT.
+
+Definition WFValueC
+           {V LT}
+           `{FunctorLaws V} `{FunctorLaws LT}
+           (WT : (WellTypedValue V LT)-indexedProp)
+           v lt
+  : Prop
+  := WFValue V LT WT (MkWellTypedValue V LT _ _ _ _ v lt).
+
+(**
+This is the most abstract statement of the type soundness of evaluation.
+
+Instead of explicitly calling recursively [evalL] and [typeOfL], this is
+abstracted over the operation to run recursively, namely [recEval] and
+[recTypeOf].
+
+ *)
+
+Definition eval_alg_Soundness_P
+           {L L' LT V}
+           `{FunctorLaws L} `{FunctorLaws L'} `{FunctorLaws LT} `{FunctorLaws V}
+           (WT : (WellTypedValue V LT -> Prop) -> WellTypedValue V LT -> Prop)
+           `{evalL   : forall {T}, MixinAlgebra L  T (EvalResult   V)}
+           `{typeOfL : forall {T}, MixinAlgebra L' T (TypeOfResult LT)}
+           (recEval : UniversalPropertyF L -> EvalResult V)
+           (recTypeOf : UniversalPropertyF L' -> TypeOfResult LT)
+           (e : Fix L' * Fix L)
+           (RFUP_e : ReverseFoldUniversalProperty (fst e) /\ ReverseFoldUniversalProperty (snd e))
+  : Prop
+  :=
+    forall
+
+      (* Commenting those out temporarily to see where they are needed! *)
+
+      (* recEvalProj : forall (e : UniversalPropertyF L),
+          recEval e
+          =
+          recEval (reverseFoldWrapFix (reverseFoldUnwrapFix (proj1_sig e)))
+      *)
+
+      (* recTypeOfProj : forall (e : UniversalPropertyF L'),
+          recTypeOf e
+          =
+          recTypeOf (reverseFoldWrapFix (reverseFoldUnwrapFix (proj1_sig e)))
+      *)
+
+      (IH : forall (a : UniversalPropertyF L' * UniversalPropertyF L),
+          (forall T,
+              typeOfL recTypeOf (reverseFoldUnwrapFix (proj1_sig (fst a))) = Some T ->
+              WFValueC WT (evalL recEval (reverseFoldUnwrapFix (proj1_sig (snd a)))) T
+          ) ->
+          forall T,
+            recTypeOf (fst a) = Some T ->
+            WFValueC WT (recEval (reverseFoldWrapFix (reverseFoldUnwrapFix (proj1_sig (snd a))))) T
+      )
+    ,
+    forall (T : TypeFix LT),
+      typeOfL recTypeOf (reverseFoldUnwrapFix (fst e)) = Some T ->
+      WFValueC WT (evalL recEval (reverseFoldUnwrapFix (snd e))) T.
+
+Definition Eval_Soundness_alg_F
+           {L LT V}
+           `{FunctorLaws L} `{FunctorLaws LT} `{FunctorLaws V}
+           (WT : (WellTypedValue V LT -> Prop) -> WellTypedValue V LT -> Prop)
+           `{EvalL   : forall {T}, ProgramAlgebra L T (EvalResult V)}
+           `{TypeOfL : forall {T}, ProgramAlgebra L T (TypeOfResult LT)}
+  := forall recTypeOf recEval,
+    ProofAlgebra
+      L
+      (sig
+         (UniversalPropertyP2
+            (eval_alg_Soundness_P
+               (evalL   := fun _ => programAlgebra' EvalL)
+               (typeOfL := fun _ => programAlgebra' TypeOfL)
+               WT
+               recTypeOf recEval
+      ))).
+
+Definition eval_Soundness_P
+           {L LT V}
+           `{FunctorLaws L} `{FunctorLaws LT} `{FunctorLaws V}
+           (WT : (WellTypedValue V LT -> Prop) -> WellTypedValue V LT -> Prop)
+           `{EvalL   : forall {T}, ProgramAlgebra L T (EvalResult V)}
+           `{TypeOfL : forall {T}, ProgramAlgebra L T (TypeOfResult LT)}
+           (recEval : UniversalPropertyF L -> EvalResult V)
+           (recTypeOf : UniversalPropertyF L -> TypeOfResult LT)
+           (e : Fix L)
+           (RFUP_e : ReverseFoldUniversalProperty e)
+  : Prop
+  :=
+    forall (T : TypeFix LT),
+      typeOf e = Some T ->
+      WFValueC WT (eval e) T.
+
+Lemma eval_Soundness
+      {L LT V}
+      `{FunctorLaws L} `{FunctorLaws LT} `{FunctorLaws V}
+      (WT : (WellTypedValue V LT -> Prop) -> WellTypedValue V LT -> Prop)
+      `{EvalL   : forall {T}, ProgramAlgebra L T (EvalResult V)}
+      `{TypeOfL : forall {T}, ProgramAlgebra L T (TypeOfResult LT)}
+      `{WFEvalL : ! WellFormedMendlerAlgebra (@EvalL)}
+      (eval_Soundness_alg_F : Eval_Soundness_alg_F WT)
+      (WF_eval_Soundness_alg_F :
+         forall recTypeOf recEval,
+           WellFormedProofAlgebra2 (eval_Soundness_alg_F recTypeOf recEval)
+      )
+  : forall (e : WellFormedValue L) (T : TypeFix LT),
+    typeOf (proj1_sig e) = Some T ->
+    WFValueC WT (eval (proj1_sig e)) T.
+Proof.
+  move => e T TO.
+  setoid_rewrite <- reverseFoldWrapUnwrapFix_inverse.
+  {
+    rewrite // / eval / mendlerFold / reverseFoldWrapFix / wrapFix /=.
+    setoid_rewrite wellFormedMendlerAlgebra.
+    rewrite / mendlerFold.
+    elim (
+        Induction2
+          (PA :=
+             eval_Soundness_alg_F
+               (fun e => eval (proj1_sig e))
+               (fun e => typeOf (proj1_sig e))
+          )
+          _
+          (proj2_sig e)
+      ).
+    rewrite / eval_alg_Soundness_P.
+    move => e' E'.
+    eapply E'.
+    move => [[f F][g G]].
+    rewrite reverseFoldWrapUnwrapFix_inverse /=.
+    rewrite / eval / mendlerFold / reverseFoldUnwrapFix / programAlgebra'.
+    admit.
+Admitted.
